fstar/MLS.TreeCommon.Lemmas.fst
@@ -28,3 +28,40 @@ val find_empty_leaf_tree_extend: #leaf_t:Type -> #node_t:Type -> #l:nat -> t:tre
   (Some? (find_empty_leaf (tree_extend t)))
 let find_empty_leaf_tree_extend #leaf_t #node_t #l t =
   find_empty_leaf_mk_blank_tree #leaf_t #node_t l (right_index #(l+1) 0)
+
+val leaf_at_tree_change_path: #leaf_t:Type -> #node_t:Type -> #l:nat -> #i:tree_index l -> t:tree leaf_t node_t l i -> li:leaf_index l i -> leaf_content:leaf_t -> node_content:node_t -> li':leaf_index l i -> Lemma
+  (leaf_at (tree_change_path t li leaf_content node_content) li' == (if li = li' then leaf_content else leaf_at t li'))
+let rec leaf_at_tree_change_path #leaf_t #node_t #l #i t li leaf_content node_content li' =
+  match t with
+  | TLeaf _ -> ()
+  | TNode _ left right -> (
+    match is_left_leaf li, is_left_leaf li' with
+    | true, true -> leaf_at_tree_change_path left li leaf_content node_content li'
+    | false, false -> leaf_at_tree_change_path right li leaf_content node_content li'
+    | _, _ -> ()
+  )
+
+val leaf_at_tree_update: #leaf_t:Type -> #node_t:Type -> #l:nat -> #i:tree_index l -> t:tree (option leaf_t) (option node_t) l i -> li:leaf_index l i -> leaf_content:leaf_t -> li':leaf_index l i -> Lemma
+  (leaf_at (tree_update t li leaf_content) li' == (if li = li' then Some leaf_content else leaf_at t li'))
+let leaf_at_tree_update #leaf_t #node_t #l #i t li leaf_content li' =
+  leaf_at_tree_change_path t li (Some leaf_content) None li'
+
+val leaf_at_tree_remove: #leaf_t:Type -> #node_t:Type -> #l:nat -> #i:tree_index l -> t:tree (option leaf_t) (option node_t) l i -> li:leaf_index l i -> li':leaf_index l i -> Lemma
+  (leaf_at (tree_remove t li) li' == (if li = li' then None else leaf_at t li'))
+let leaf_at_tree_remove #leaf_t #node_t #l #i t li li' =
+  leaf_at_tree_change_path t li None None li'
+
+val leaf_at_mk_blank_tree_general: #leaf_t:Type -> #node_t:Type -> l:nat -> i:tree_index l -> leaf_content:leaf_t -> node_content:node_t -> li':leaf_index l i -> Lemma
+  (leaf_at (mk_blank_tree_general #leaf_t #node_t l i leaf_content node_content) li' == leaf_content)
+let rec leaf_at_mk_blank_tree_general #leaf_t #node_t l i leaf_content node_content li' =
+  if l = 0 then ()
+  else if is_left_leaf li' then
+    leaf_at_mk_blank_tree_general (l-1) (left_index i) leaf_content node_content li'
+  else
+    leaf_at_mk_blank_tree_general (l-1) (right_index i) leaf_content node_content li'
+
+val leaf_at_tree_extend: #leaf_t:Type -> #node_t:Type -> #l:nat -> t:tree (option leaf_t) (option node_t) l 0 -> li':leaf_index (l+1) 0 -> Lemma
+  (leaf_at (tree_extend t) li' == (if li' < pow2 l then leaf_at t li' else None))
+let leaf_at_tree_extend #leaf_t #node_t #l t li' =
+  if li' < pow2 l then ()
+  else leaf_at_mk_blank_tree_general #(option leaf_t) #(option node_t) l (right_index #(l+1) 0) None None li'
