fstar/MLS.TreeSync.API.Types.fst
@@ -5,13 +5,16 @@ open MLS.Crypto
 open MLS.NetworkTypes
 open MLS.TreeSync.NetworkTypes
 open MLS.TreeSync.Refined.Types
+open MLS.TreeSync.Invariants.AuthService
 
 (** TreeSync state and accessors *)
-type treesync_state (bytes:Type0) {|crypto_bytes bytes|} (tkt:treekem_types bytes) = {
+noeq
+type treesync_state (bytes:Type0) {|crypto_bytes bytes|} (tkt:treekem_types bytes) (asp:as_parameters bytes) = {
   group_id: mls_bytes bytes;
   levels: nat;
   tree: treesync_valid bytes tkt levels 0 group_id;
+  tokens: tokens:Ghost.erased (as_tokens bytes asp levels 0){all_credentials_ok tree tokens};
   version: nat;
 }
 
-type treesync_index (#bytes:Type0) {|crypto_bytes bytes|} (#tkt:treekem_types bytes) (st:treesync_state bytes tkt) = i:nat{i < pow2 st.levels}
+type treesync_index (#bytes:Type0) {|crypto_bytes bytes|} (#tkt:treekem_types bytes) (#asp:as_parameters bytes) (st:treesync_state bytes tkt asp) = i:nat{i < pow2 st.levels}
