fstar/MLS.TreeSync.API.fst
@@ -2,9 +2,11 @@ module MLS.TreeSync.API
 
 open Comparse
 open MLS.Crypto
+open MLS.MiscLemmas
 open MLS.NetworkTypes
 open MLS.TreeSync.NetworkTypes
 open MLS.Tree
+open MLS.Tree.Lemmas
 open MLS.TreeCommon
 open MLS.TreeCommon.Lemmas
 open MLS.TreeSync.Types
@@ -12,93 +14,437 @@ open MLS.TreeSync.Operations
 open MLS.TreeSync.Refined.Types
 open MLS.TreeSync.Refined.Operations
 open MLS.TreeSync.API.Types
+open MLS.TreeSync.Invariants.UnmergedLeaves
+open MLS.TreeSync.Invariants.ParentHash
+open MLS.TreeSync.Invariants.ValidLeaves
+open MLS.TreeSync.Invariants.AuthService
+open MLS.TreeSync.Invariants.AuthService.Proofs
 open MLS.Result
 
 #set-options "--fuel 0 --ifuel 0"
 
-#push-options "--fuel 1 --ifuel 1"
-val create: #bytes:Type0 -> {|crypto_bytes bytes|} -> #tkt:treekem_types bytes -> group_id:mls_bytes bytes -> ln:leaf_node_nt bytes tkt -> result (treesync_state bytes tkt)
-let create #bytes #cb group_id ln =
-  if not (leaf_is_valid ln group_id 0) then
-    error "create: leaf node is not valid"
-  else (
-    return ({
-      group_id;
-      levels = 0;
-      tree = tree_create (Some ln);
-      version = 0;
-    })
-  )
-#pop-options
+let as_input_for (#bytes:Type0) {|bytes_like bytes|} (#tkt:treekem_types bytes) (ln:leaf_node_nt bytes tkt) =
+  x:as_input bytes{ x == leaf_node_to_as_input ln }
 
-val state_update_tree: #bytes:Type0 -> {|crypto_bytes bytes|} -> #tkt:treekem_types bytes -> #l:nat -> st:treesync_state bytes tkt -> treesync_valid bytes tkt l 0 st.group_id -> treesync_state bytes tkt
-let state_update_tree #bytes #cb #tkt #l st new_tree =
+let as_token_for (#bytes:Type0) {|bytes_like bytes|} (asp:as_parameters bytes) (inp:as_input bytes) =
+  token:asp.token_t{ asp.credential_ok inp token }
+
+val state_leaf_at: #bytes:Type0 -> {|crypto_bytes bytes|} -> #tkt:treekem_types bytes -> #asp:as_parameters bytes -> st:treesync_state bytes tkt asp -> li:treesync_index st{Some? (leaf_at st.tree li)} -> leaf_node_nt bytes tkt
+let state_leaf_at #bytes #cb #tkt #asp st li =
+  Some?.v (leaf_at st.tree li)
+
+val state_update_tree:
+  #bytes:Type0 -> {|crypto_bytes bytes|} -> #tkt:treekem_types bytes -> #asp:as_parameters bytes -> #l:nat ->
+  st:treesync_state bytes tkt asp -> new_tree:treesync_valid bytes tkt l 0 st.group_id -> new_tokens:Ghost.erased (as_tokens bytes asp l 0){all_credentials_ok new_tree new_tokens} ->
+  treesync_state bytes tkt asp
+let state_update_tree #bytes #cb #tkt #asp #l st new_tree new_tokens =
   ({ st with
     levels = l;
     version = st.version + 1;
     tree = new_tree;
+    tokens = new_tokens;
   })
 
-val get_leaf_package_from_key_package: #bytes:Type0 -> {|crypto_bytes bytes|} -> #tkt:treekem_types bytes -> key_package_nt bytes tkt -> result (leaf_node_nt bytes tkt)
-let get_leaf_package_from_key_package #bytes #cb kp =
-  //TODO check signature
-  if not (kp.tbs.leaf_node.data.source = LNS_key_package ()) then
-    error "get_leaf_package_from_key_package: source is not add"
-  else (
-    return kp.tbs.leaf_node
+(*** Create ***)
+
+let pending_create_proof (#bytes:Type0) {|crypto_bytes bytes|} (#tkt:treekem_types bytes) (group_id:mls_bytes bytes) (ln:leaf_node_nt bytes tkt) =
+  squash (
+    leaf_is_valid ln group_id 0
   )
 
-val add: #bytes:Type0 -> {|crypto_bytes bytes|} -> #tkt:treekem_types bytes -> treesync_state bytes tkt -> key_package_nt bytes tkt -> result (treesync_state bytes tkt & nat)
-let add #bytes #cb #tkt st kp =
-  ln <-- get_leaf_package_from_key_package kp;
-  if not (ln.data.source = LNS_key_package()) then
-    error "add: bad leaf node source"
+type pending_create (#bytes:Type0) {|crypto_bytes bytes|} (#tkt:treekem_types bytes) (group_id:mls_bytes bytes) (ln:leaf_node_nt bytes tkt) = {
+  can_create_proof: pending_create_proof group_id ln;
+  as_input: as_input_for ln;
+}
+
+type token_for_create
+  (#bytes:Type0) {|crypto_bytes bytes|} (#tkt:treekem_types bytes)
+  (#group_id:mls_bytes bytes) (#ln:leaf_node_nt bytes tkt)
+  (asp:as_parameters bytes) (pend:pending_create group_id ln) =
+  as_token_for asp pend.as_input
+
+val prepare_create:
+  #bytes:Type0 -> {|crypto_bytes bytes|} -> #tkt:treekem_types bytes ->
+  group_id:mls_bytes bytes -> ln:leaf_node_nt bytes tkt ->
+  result (pending_create group_id ln)
+let prepare_create #bytes #cb #tkt group_id ln =
+  if not (leaf_is_valid ln group_id 0) then
+    error "prepare_create: leaf node is not valid"
   else (
-    match find_empty_leaf st.tree with
-    | Some i ->
-      if not (tree_add_pre st.tree i) then
-        error "add: tree_add_pre is false"
-      else if not (leaf_is_valid ln st.group_id i) then
-        error "add: invalid leaf node"
-      else
-        return (state_update_tree st (tree_add st.tree i ln), (i <: nat))
-    | None ->
-      find_empty_leaf_tree_extend st.tree;
-      let extended_tree = tree_extend st.tree in
-      let i = Some?.v (find_empty_leaf extended_tree) in
-      if not (tree_add_pre extended_tree i) then
-        error "add: tree_add_pre is false (after extension)"
-      else if not (leaf_is_valid ln st.group_id i) then
-        error "add: invalid leaf node"
-      else
-        return (state_update_tree st (tree_add extended_tree i ln), (i <: nat))
+    return ({
+      can_create_proof = ();
+      as_input = leaf_node_to_as_input ln;
+    })
   )
 
-val update: #bytes:Type0 -> {|crypto_bytes bytes|} -> #tkt:treekem_types bytes -> st:treesync_state bytes tkt -> leaf_node_nt bytes tkt -> treesync_index st -> result (treesync_state bytes tkt)
-let update #bytes #cb #tkt st ln i =
-  if not (ln.data.source = LNS_update()) then
-    error "update: leaf node has invalid source"
-  else if not (leaf_is_valid ln st.group_id i) then
-    error "update: leaf node is not valid"
-  else (
-    return (state_update_tree st (tree_update st.tree i ln))
+#push-options "--fuel 1 --ifuel 1"
+val finalize_create:
+  #bytes:Type0 -> {|crypto_bytes bytes|} -> #tkt:treekem_types bytes -> #asp:as_parameters bytes ->
+  #group_id:mls_bytes bytes -> #ln:leaf_node_nt bytes tkt ->
+  pend:pending_create group_id ln -> token:token_for_create asp pend ->
+  treesync_state bytes tkt asp
+let finalize_create #bytes #cb #tkt #asp #group_id #ln pend token =
+  ({
+    group_id;
+    levels = 0;
+    tree = tree_create (Some ln);
+    tokens = tree_create (Some token);
+    version = 0;
+  })
+#pop-options
+
+(*** Welcome ***)
+
+let pending_welcome_proof (#bytes:Type0) {|crypto_bytes bytes|} (#tkt:treekem_types bytes) (#l:nat) (group_id:mls_bytes bytes) (t:treesync bytes tkt l 0) (version:nat) = 
+  squash (
+    unmerged_leaves_ok t /\
+    parent_hash_invariant t /\
+    valid_leaves_invariant group_id t
   )
 
 #push-options "--fuel 0 --ifuel 1"
-val remove: #bytes:Type0 -> {|crypto_bytes bytes|} -> #tkt:treekem_types bytes -> st:treesync_state bytes tkt -> i:treesync_index st -> treesync_state bytes tkt
-let remove #bytes #cb #tkt st i =
-  let blanked_tree = (tree_remove st.tree i) in
-  if TNode? blanked_tree && is_tree_empty (TNode?.right blanked_tree) then
-    state_update_tree st (tree_truncate blanked_tree)
-  else
-    state_update_tree st blanked_tree
+type pending_welcome (#bytes:Type0) {|crypto_bytes bytes|} (#tkt:treekem_types bytes) (#l:nat) (group_id:mls_bytes bytes) (t:treesync bytes tkt l 0) (version:nat) = {
+  can_welcome_proof: pending_welcome_proof group_id t version;
+  as_inputs: list (option (as_input bytes));
+  as_inputs_proof: squash (
+    List.Tot.length as_inputs == pow2 l /\ (
+      forall (li:nat{li < pow2 l}). List.Tot.index as_inputs li == Option.mapTot leaf_node_to_as_input (leaf_at t li)
+    )
+  );
+}
 #pop-options
 
-val commit: #bytes:Type0 -> {|crypto_bytes bytes|} -> #tkt:treekem_types bytes -> st:treesync_state bytes tkt -> #li:treesync_index st -> pathsync bytes tkt st.levels 0 li -> result (treesync_state bytes tkt)
-let commit #bytes #cb #tkt st #li p =
+type tokens_for_welcome
+  (#bytes:Type0) {|crypto_bytes bytes|} (#tkt:treekem_types bytes) (#l:nat)
+  (#group_id:mls_bytes bytes) (#t:treesync bytes tkt l 0) (#version:nat)
+  (asp:as_parameters bytes) (pend:pending_welcome group_id t version) =
+  tokens:list (option asp.token_t){
+    List.Tot.length tokens == pow2 l /\ (
+      forall li. match List.Tot.index pend.as_inputs li, List.Tot.index tokens li with
+      | Some as_inp, Some token -> asp.credential_ok as_inp token
+      | None, None -> True
+      | _, _ -> False
+    )
+  }
+
+val prepare_welcome:
+  #bytes:Type0 -> {|crypto_bytes bytes|} -> #tkt:treekem_types bytes -> #l:nat ->
+  group_id:mls_bytes bytes -> t:treesync bytes tkt l 0 -> version:nat ->
+  result (pending_welcome group_id t version)
+let prepare_welcome #bytes #cb #tkt #l group_id t version =
+  if not (unmerged_leaves_ok t) then
+    error "prepare_welcome: malformed unmerged leaves"
+  else if not (parent_hash_invariant t) then
+    error "prepare_welcome: bad parent hash"
+  else if not (valid_leaves_invariant group_id t) then
+    error "prepare_welcome: invalid leaves"
+  else (
+    let as_inputs = List.Tot.map (Option.mapTot leaf_node_to_as_input) (get_leaf_list t) in
+    introduce forall (li:nat{li < pow2 l}). List.Tot.index as_inputs li == Option.mapTot leaf_node_to_as_input (leaf_at t li)
+    with (
+      index_get_leaf_list t li;
+      index_map (Option.mapTot leaf_node_to_as_input) (get_leaf_list t) li
+    );
+    return ({
+      can_welcome_proof = ();
+      as_inputs;
+      as_inputs_proof = ();
+    })
+  )
+
+#push-options "--fuel 2 --ifuel 2"
+val tokens_from_list: #bytes:Type0 -> {|bytes_like bytes|} -> asp:as_parameters bytes -> l:nat -> i:tree_index l -> tokens:list (option asp.token_t){List.Tot.length tokens == pow2 l} -> as_tokens bytes asp l i
+let rec tokens_from_list #bytes #bl asp l i tokens =
+  if l = 0 then (
+    let [token] = tokens in
+    TLeaf token
+  ) else (
+    let tokens_left, tokens_right = List.Tot.splitAt (pow2 (l-1)) tokens in
+    List.Pure.splitAt_length (pow2 (l-1)) tokens;
+    TNode () (tokens_from_list asp _ _ tokens_left) (tokens_from_list asp _ _ tokens_right)
+  )
+#pop-options
+
+#push-options "--fuel 2 --ifuel 2"
+val leaf_at_token_from_list: #bytes:Type0 -> {|bytes_like bytes|} -> asp:as_parameters bytes -> l:nat -> i:tree_index l -> tokens:list (option asp.token_t){List.Tot.length tokens == pow2 l} -> li:leaf_index l i -> Lemma (
+  leaf_at (tokens_from_list asp l i tokens) li == List.Tot.index tokens (li-i)
+)
+let rec leaf_at_token_from_list #bytes #bl asp l i tokens li =
+  if l = 0 then ()
+  else (
+    let tokens_left, tokens_right = List.Tot.splitAt (pow2 (l-1)) tokens in
+    List.Pure.lemma_splitAt tokens tokens_left tokens_right (pow2 (l-1));
+    index_append tokens_left tokens_right (li-i);
+    if is_left_leaf li then
+      leaf_at_token_from_list asp (l-1) (left_index i) tokens_left li
+    else
+      leaf_at_token_from_list asp (l-1) (right_index i) tokens_right li
+  )
+#pop-options
+
+val finalize_welcome:
+  #bytes:Type0 -> {|crypto_bytes bytes|} -> #tkt:treekem_types bytes -> #asp:as_parameters bytes -> #l:nat ->
+  #group_id:mls_bytes bytes -> #t:treesync bytes tkt l 0 -> #version:nat ->
+  pend:pending_welcome group_id t version -> tokens:tokens_for_welcome asp pend ->
+  treesync_state bytes tkt asp
+let finalize_welcome #bytes #cb #tkt #asp #l #group_id #t #version pend tokens =
+  pend.can_welcome_proof;
+  let tokens_tree = tokens_from_list asp l 0 tokens in
+  intro_all_credentials_ok t tokens_tree (fun li ->
+    pend.as_inputs_proof;
+    leaf_at_token_from_list asp l 0 tokens li
+  );
+  ({
+    group_id;
+    levels = l;
+    tree = t;
+    tokens = tokens_tree;
+    version;
+  })
+
+(*** Add ***)
+
+let pending_add_proof (#bytes:Type0) {|crypto_bytes bytes|} (#tkt:treekem_types bytes) (#asp:as_parameters bytes) (st:treesync_state bytes tkt asp) (kp:key_package_nt bytes tkt) =
+  squash (
+    kp.tbs.leaf_node.data.source == LNS_key_package () /\
+    True /\ ( //TODO: check key package signature
+      match find_empty_leaf st.tree with
+      | Some li ->
+        tree_add_pre st.tree li /\
+        leaf_is_valid kp.tbs.leaf_node st.group_id li
+      | None ->
+        find_empty_leaf_tree_extend st.tree;
+        let extended_tree = tree_extend st.tree in
+        let li = Some?.v (find_empty_leaf extended_tree) in
+        tree_add_pre extended_tree li /\
+        leaf_is_valid kp.tbs.leaf_node st.group_id li
+    )
+  )
+
+type pending_add (#bytes:Type0) {|crypto_bytes bytes|} (#tkt:treekem_types bytes) (#asp:as_parameters bytes) (st:treesync_state bytes tkt asp) (kp:key_package_nt bytes tkt) = {
+  can_add_proof: pending_add_proof st kp;
+  as_input: as_input_for kp.tbs.leaf_node;
+}
+
+type token_for_add
+  (#bytes:Type0) {|crypto_bytes bytes|} (#tkt:treekem_types bytes) (#asp:as_parameters bytes)
+  (#st:treesync_state bytes tkt asp) (#kp:key_package_nt bytes tkt)
+  (pend:pending_add st kp) =
+  as_token_for asp pend.as_input
+
+val prepare_add:
+  #bytes:Type0 -> {|crypto_bytes bytes|} -> #tkt:treekem_types bytes -> #asp:as_parameters bytes ->
+  st:treesync_state bytes tkt asp -> kp:key_package_nt bytes tkt ->
+  result (pending_add st kp)
+let prepare_add #bytes #cb #tkt #asp st kp =
+  if not (kp.tbs.leaf_node.data.source = LNS_key_package ()) then
+    error "prepare_add: source is not key_package"
+  else (
+    let ln = kp.tbs.leaf_node in
+    match find_empty_leaf st.tree with
+    | Some li ->
+      if not (tree_add_pre st.tree li) then
+        error "prepare_add: tree_add_pre is false"
+      else if not (leaf_is_valid ln st.group_id li) then
+        error "prepare_add: invalid leaf node"
+      else (
+        return ({
+          can_add_proof = ();
+          as_input = leaf_node_to_as_input ln;
+        })
+      )
+    | None ->
+      find_empty_leaf_tree_extend st.tree;
+      let extended_tree = tree_extend st.tree in
+      let li = Some?.v (find_empty_leaf extended_tree) in
+      if not (tree_add_pre extended_tree li) then
+        error "prepare_add: tree_add_pre is false (after extension)"
+      else if not (leaf_is_valid ln st.group_id li) then
+        error "prepare_add: invalid leaf node"
+      else (
+        return ({
+          can_add_proof = ();
+          as_input = leaf_node_to_as_input ln;
+        })
+      )
+  )
+
+val finalize_add:
+  #bytes:Type0 -> {|crypto_bytes bytes|} -> #tkt:treekem_types bytes -> #asp:as_parameters bytes ->
+  #st:treesync_state bytes tkt asp -> #kp:key_package_nt bytes tkt ->
+  pend:pending_add st kp -> token:token_for_add pend ->
+  treesync_state bytes tkt asp & nat
+let finalize_add #bytes #cb #tkt #asp #st #kp pend token =
+  pend.can_add_proof;
+  let ln = kp.tbs.leaf_node in
+  match find_empty_leaf st.tree with
+  | Some li -> (
+    all_credentials_ok_tree_add st.tree st.tokens li ln token;
+    (state_update_tree st (tree_add st.tree li ln) (as_add_update st.tokens li token), (li <: nat))
+  )
+  | None -> (
+    find_empty_leaf_tree_extend st.tree;
+    let extended_tree = tree_extend st.tree in
+    let extended_tokens = Ghost.hide (as_extend st.tokens) in
+    let li = Some?.v (find_empty_leaf extended_tree) in
+    all_credentials_ok_tree_extend st.tree st.tokens;
+    all_credentials_ok_tree_add extended_tree extended_tokens li ln token;
+    (state_update_tree st (tree_add extended_tree li ln) (as_add_update extended_tokens li token), (li <: nat))
+)
+
+(*** Update ***)
+
+let pending_update_proof (#bytes:Type0) {|crypto_bytes bytes|} (#tkt:treekem_types bytes) (#asp:as_parameters bytes) (st:treesync_state bytes tkt asp) (ln:leaf_node_nt bytes tkt) (li:treesync_index st) =
+  squash (
+    ln.data.source == LNS_update () /\
+    leaf_is_valid ln st.group_id li /\
+    Some? (leaf_at st.tree li)
+  )
+
+type pending_update (#bytes:Type0) {|crypto_bytes bytes|} (#tkt:treekem_types bytes) (#asp:as_parameters bytes) (st:treesync_state bytes tkt asp) (ln:leaf_node_nt bytes tkt) (li:treesync_index st) = {
+  can_update_proof: pending_update_proof st ln li;
+  as_input_before: (can_update_proof; as_input_for (state_leaf_at st li));
+  as_input: as_input_for ln;
+}
+
+type token_for_update
+  (#bytes:Type0) {|crypto_bytes bytes|} (#tkt:treekem_types bytes) (#asp:as_parameters bytes)
+  (#st:treesync_state bytes tkt asp) (#ln:leaf_node_nt bytes tkt) (#li:treesync_index st)
+  (pend:pending_update st ln li) =
+  token:as_token_for asp pend.as_input{asp.valid_successor pend.as_input_before pend.as_input}
+
+val prepare_update:
+  #bytes:Type0 -> {|crypto_bytes bytes|} -> #tkt:treekem_types bytes -> #asp:as_parameters bytes ->
+  st:treesync_state bytes tkt asp -> ln:leaf_node_nt bytes tkt -> li:treesync_index st ->
+  result (pending_update st ln li)
+let prepare_update #bytes #cb #tkt #asp st ln li =
+  if not (ln.data.source = LNS_update()) then
+    error "prepare_update: leaf node has invalid source"
+  else if not (leaf_is_valid ln st.group_id li) then
+    error "prepare_update: leaf node is not valid"
+  else if not (Some? (leaf_at st.tree li)) then
+    error "prepare_update: leaf node doesn't exists"
+  else (
+    return ({
+      can_update_proof = ();
+      as_input_before = leaf_node_to_as_input (state_leaf_at st li);
+      as_input = leaf_node_to_as_input ln;
+    })
+  )
+
+val finalize_update:
+  #bytes:Type0 -> {|crypto_bytes bytes|} -> #tkt:treekem_types bytes -> #asp:as_parameters bytes ->
+  #st:treesync_state bytes tkt asp -> #ln:leaf_node_nt bytes tkt -> #li:treesync_index st ->
+  pend:pending_update st ln li -> token:token_for_update pend ->
+  treesync_state bytes tkt asp
+let finalize_update #bytes #cb #tkt #asp #st #ln #li pend token =
+  pend.can_update_proof;
+  all_credentials_ok_tree_update st.tree st.tokens li ln token;
+  (state_update_tree st (tree_update st.tree li ln) (as_add_update st.tokens li token))
+
+(*** Remove ***)
+
+let pending_remove_proof (#bytes:Type0) {|crypto_bytes bytes|} (#tkt:treekem_types bytes) (#asp:as_parameters bytes) (st:treesync_state bytes tkt asp) (li:treesync_index st) =
+  squash (
+    Some? (leaf_at st.tree li)
+  )
+
+type pending_remove (#bytes:Type0) {|crypto_bytes bytes|} (#tkt:treekem_types bytes) (#asp:as_parameters bytes) (st:treesync_state bytes tkt asp) (li:treesync_index st) = {
+  can_remove_proof: pending_remove_proof st li;
+}
+
+val prepare_remove:
+  #bytes:Type0 -> {|crypto_bytes bytes|} -> #tkt:treekem_types bytes -> #asp:as_parameters bytes ->
+  st:treesync_state bytes tkt asp -> li:treesync_index st ->
+  result (pending_remove st li)
+let prepare_remove #bytes #cb #tkt st li =
+  if not (Some? (leaf_at st.tree li)) then
+    error "prepare_remove: removed leaf is already blank"
+  else (
+    return ({
+      can_remove_proof = ();
+    })
+  )
+
+#push-options "--fuel 0 --ifuel 1"
+val finalize_remove:
+  #bytes:Type0 -> {|crypto_bytes bytes|} -> #tkt:treekem_types bytes -> #asp:as_parameters bytes ->
+  #st:treesync_state bytes tkt asp -> #li:treesync_index st ->
+  pend:pending_remove st li ->
+  treesync_state bytes tkt asp
+let finalize_remove #bytes #cb #tkt #asp #st #li pend =
+  let blanked_tree = (tree_remove st.tree li) in
+  let blanked_tokens = Ghost.hide (as_remove st.tokens li) in
+  all_credentials_ok_tree_remove st.tree st.tokens li;
+  if TNode? blanked_tree && is_tree_empty (TNode?.right blanked_tree) then (
+    all_credentials_ok_tree_truncate blanked_tree blanked_tokens;
+    state_update_tree st (tree_truncate blanked_tree) (as_truncate blanked_tokens)
+  ) else (
+    state_update_tree st blanked_tree blanked_tokens
+  )
+#pop-options
+
+(*** Commit ***)
+
+let pending_commit_proof (#bytes:Type0) {|crypto_bytes bytes|} (#tkt:treekem_types bytes) (#asp:as_parameters bytes) (st:treesync_state bytes tkt asp) (#li:treesync_index st) (p:pathsync bytes tkt st.levels 0 li) =
+  squash (
+    apply_path_pre st.tree p /\
+    path_is_valid st.group_id st.tree p /\
+    Some? (leaf_at st.tree li)
+  )
+
+#push-options "--fuel 0 --ifuel 1"
+type pending_commit (#bytes:Type0) {|crypto_bytes bytes|} (#tkt:treekem_types bytes) (#asp:as_parameters bytes) (st:treesync_state bytes tkt asp) (#li:treesync_index st) (p:pathsync bytes tkt st.levels 0 li) = {
+  can_commit_proof: pending_commit_proof st p;
+  as_input_before: (can_commit_proof; as_input_for (state_leaf_at st li));
+  as_input: as_input_for (get_path_leaf p);
+}
+#pop-options
+
+type token_for_commit
+  (#bytes:Type0) {|crypto_bytes bytes|} (#tkt:treekem_types bytes) (#asp:as_parameters bytes)
+  (#st:treesync_state bytes tkt asp) (#li:treesync_index st) (#p:pathsync bytes tkt st.levels 0 li)
+  (pend:pending_commit st p) =
+  token:as_token_for asp pend.as_input{asp.valid_successor pend.as_input_before pend.as_input}
+
+val prepare_commit:
+  #bytes:Type0 -> {|crypto_bytes bytes|} -> #tkt:treekem_types bytes -> #asp:as_parameters bytes ->
+  st:treesync_state bytes tkt asp -> #li:treesync_index st -> p:pathsync bytes tkt st.levels 0 li ->
+  result (pending_commit st p)
+let prepare_commit #bytes #cb #tkt #asp st #li p =
   if not (apply_path_pre st.tree p) then
-    error "commit: bad precondition"
+    error "prepare_commit: bad precondition"
   else if not (path_is_valid st.group_id st.tree p) then
-    error "commit: invalid path"
-  else
-    return (state_update_tree st (apply_path st.tree p))
+    error "prepare_commit: invalid path"
+  else if not (Some? (leaf_at st.tree li)) then
+    error "prepare_commit: comitter is blank"
+  else (
+    return ({
+      can_commit_proof = ();
+      as_input_before = leaf_node_to_as_input (state_leaf_at st li);
+      as_input = leaf_node_to_as_input (get_path_leaf p);
+    })
+  )
+
+#push-options "--fuel 0 --ifuel 1"
+val finalize_commit:
+  #bytes:Type0 -> {|crypto_bytes bytes|} -> #tkt:treekem_types bytes -> #asp:as_parameters bytes ->
+  #st:treesync_state bytes tkt asp -> #li:treesync_index st -> #p:pathsync bytes tkt st.levels 0 li ->
+  pend:pending_commit st p -> token:token_for_commit pend ->
+  treesync_state bytes tkt asp
+let finalize_commit #bytes #cb #tkt #asp #st #li #p pend token =
+  pend.can_commit_proof;
+  all_credentials_ok_apply_path st.tree st.tokens p token;
+  state_update_tree st (apply_path st.tree p) (as_add_update st.tokens li token)
+#pop-options
+
+(*** Weaken ***)
+
+val weaken_asp:
+  #bytes:Type0 -> {|crypto_bytes bytes|} -> #tkt:treekem_types bytes -> #asp:as_parameters bytes ->
+  asp_weak:as_parameters bytes{as_parameters_weaker asp asp_weak} -> treesync_state bytes tkt asp ->
+  treesync_state bytes tkt asp_weak
+let weaken_asp #bytes #cb #tkt #asp asp_weak st =
+  { st with
+    tokens = all_credentials_ok_weaken asp_weak st.tree st.tokens;
+  }
